Example 2 - Isolation buffer

theories/examples/buffer_isolation.v
@@ -9,11 +9,11 @@ From cap_machine.examples Require Export template_adequacy_concurrency.
 From iris.program_logic Require Import adequacy.
 Open Scope Z_scope.
 
-Section shared_buffer.
+Section buffer.
   Context {Σ:gFunctors} {memg:memG Σ} {regg:regG Σ}
           `{MP: MachineParameters}.
 
-  Definition buffer_code1 (b_buf e_buf: Addr) : list Word :=
+  Definition buffer_code (b_buf e_buf: Addr) : list Word :=
     (* code: *)
     encodeInstrsW [
       Mov r_t1 PC;
@@ -25,60 +25,27 @@ Section shared_buffer.
       Jmp r_t0
     ].
 
-  Definition data1 (b_buf e_buf: Addr) : list Word  :=
+  Definition data (b_buf e_buf: Addr) : list Word  :=
       [ WCap RWX b_buf e_buf (b_buf ^+ 3)%a ].
 
-  Definition buffer_prog1 a_first b_buf e_buf :=
-    ([∗ list] a_i;w ∈ a_first;(buffer_code1 b_buf e_buf) ++ (data1 b_buf e_buf), a_i ↦ₐ w)%I.
+  Definition buffer_prog a_first b_buf e_buf :=
+    ([∗ list] a_i;w ∈ a_first;(buffer_code b_buf e_buf) ++ (data b_buf e_buf), a_i ↦ₐ w)%I.
 
-  Definition buffer_code2 (b_buf e_buf: Addr) : list Word :=
-    (* code: *)
-    encodeInstrsW [
-      Mov r_t1 PC;
-      Lea r_t1 7 ;
-      Load r_t1 r_t1 ;
-      Store r_t1 (-42) ;
-      Lea r_t1 (-4);
-      Subseg r_t1 b_buf (b_buf+3)%Z;
-      Jmp r_t0
-    ].
-
-  Definition data2 (b_buf e_buf: Addr) : list Word  :=
-      [ WCap RWX b_buf e_buf (b_buf ^+ 4)%a ].
-
-  Definition buffer_prog2 a_first b_buf e_buf :=
-    ([∗ list] a_i;w ∈ a_first;(buffer_code2 b_buf e_buf) ++ (data2 b_buf e_buf), a_i ↦ₐ w)%I.
-
-  Definition secret_buffer := map WInt [ 0 ; 0].
+  Definition secret_buffer := map WInt [ 0 ].
   Definition public_buffer := map WInt [ 72 (* 'H' *); 105 (* 'i' *); 0].
-  Definition shared_buffer : list Word :=
+  Definition full_buffer : list Word :=
     public_buffer++secret_buffer.
 
 
   (** We define the invariants *)
   Definition Nsb : namespace := nroot .@ "Nshared_buffer".
 
-  (* program 1 *)
-  Definition prog1N := Nsb.@"prog1".
-  Definition prog1_inv a b_buf e_buf :=
-    inv prog1N (buffer_prog1 a b_buf e_buf).
-
-  (* program 2 *)
-  Definition prog2N := Nsb.@"prog2".
-  Definition prog2_inv a b_buf e_buf :=
-    inv prog2N (buffer_prog2 a b_buf e_buf).
-
   Definition bufferN := Nsb.@"buffer".
   Definition buffer_inv {Hinv} (b_buf e_buf : Addr) : iProp Σ :=
-   ([∗ list] a ∈ (finz.seq_between b_buf (b_buf ^+3)%a ),
-      (inv (invG0 := Hinv) (logN .@ a) (interp_ref_inv a (λne w, interp w))))%I
-      ∗ inv (invG0 := Hinv) (Nsb .@ (b_buf ^+ 3)%a)
-                 ((b_buf ^+ 3)%a ↦ₐ (WInt 0) ∨ (b_buf ^+ 3)%a ↦ₐ (WInt 42))%I
-      ∗ inv (invG0 := Hinv) (Nsb .@ (b_buf ^+ 4)%a)
-        ((b_buf ^+ 4)%a ↦ₐ (WInt 0) ∨ (b_buf ^+ 4)%a ↦ₐ (WInt (-42)))%I
-  .
+      inv (invG0 := Hinv) (Nsb .@ (b_buf ^+ 3)%a)
+                 ((b_buf ^+ 3)%a ↦ₐ (WInt 0) ∨ (b_buf ^+ 3)%a ↦ₐ (WInt 42))%I.
 
-  Lemma buffer_spec1 (i: CoreN)
+  Lemma buffer_spec (i: CoreN)
     p b e a a_first a_last
     (b_buf e_buf: Addr)
     wadv w1 φ :
@@ -86,34 +53,33 @@ Section shared_buffer.
     ExecPCPerm p →
     SubBounds b e a_first a_last ->
     contiguous_between a a_first a_last →
-    e_buf = (b_buf ^+ (length shared_buffer))%a ->
-    (b_buf ^+ 3 < e_buf)%a →
-    (b_buf ^+ 4 < e_buf)%a →
+    e_buf = (b_buf ^+ (length full_buffer))%a ->
+    (b_buf ^+ 3)%a < e_buf ->
 
    ⊢ (( (i, PC) ↦ᵣ WCap p b e a_first
       ∗ (i, r_t0) ↦ᵣ wadv
       ∗ (i, r_t1) ↦ᵣ w1
-      ∗ buffer_prog1 a b_buf e_buf
+      ∗ buffer_prog a b_buf e_buf
       ∗ buffer_inv b_buf e_buf
       ∗ ▷ ((i, PC) ↦ᵣ updatePcPerm wadv
            ∗ (i, r_t0) ↦ᵣ wadv
            ∗ (i, r_t1) ↦ᵣ WCap RWX b_buf (b_buf ^+ 3)%a b_buf%a
-           ∗ buffer_prog1 a b_buf e_buf
+           ∗ buffer_prog a b_buf e_buf
            ∗ buffer_inv b_buf e_buf
            -∗ WP (i, Seq (Instr Executable)) {{ φ }}))
       -∗ WP (i, Seq (Instr Executable)) {{ φ }})%I.
   Proof.
-    iIntros (HPCperm HPCbounds Hcont He_buf Hsecret1 Hsecret2)
-      "(HPC & Hr0 & Hr1 & Hprog & #(Hbuffer_pub & Hsecret1_inv & Hsecret2_inv) & Hφ)" .
+    iIntros (HPCperm HPCbounds Hcont He_buf HVe_buf)
+      "(HPC & Hr0 & Hr1 & Hprog & #Hsecret_inv & Hφ)" .
     set (e_buf' := e_buf).
     rename e_buf into eb ; rename e_buf' into e_buf ; subst eb.
-    rewrite {1}/buffer_prog1.
+    rewrite {1}/buffer_prog.
 
     iDestruct (contiguous_between_program_split with "Hprog") as
-      (buffer_code data a_data) "(Hprog & Hdata & #Hcont1)"
+      (buffer_codes datas a_data) "(Hprog & Hdata & #Hcont1)"
     ;[apply Hcont|].
     iDestruct "Hcont1" as %(Hcont_code & Hcont_buffer & Heqapp1 & Ha_data).
-    rewrite /data1.
+    rewrite /data.
     iDestruct (big_sepL2_length with "Hprog") as %Hlength_code.
     iDestruct (big_sepL2_length with "Hdata") as %Hlength_data.
     simpl in Hlength_data.
@@ -123,10 +89,10 @@ Section shared_buffer.
     iDestruct ((big_sepL2_singleton (λ _ a_i w_i, (a_i ↦ₐ w_i)%I)) with "Hdata")
       as "Hdata".
 
-    iAssert (codefrag a_first (buffer_code1 b_buf e_buf)) with "[Hprog]" as "Hprog".
+    iAssert (codefrag a_first (buffer_code b_buf e_buf)) with "[Hprog]" as "Hprog".
     { rewrite /codefrag. simpl. rewrite /region_mapsto.
       simpl in *.
-      replace buffer_code with (finz.seq_between a_first (a_first ^+ 7%nat)%a).
+      replace buffer_codes with (finz.seq_between a_first (a_first ^+ 7%nat)%a).
       done.
       symmetry.
       apply region_addrs_of_contiguous_between.
@@ -139,23 +105,21 @@ Section shared_buffer.
     replace (a_first ^+ 7)%a with a_data ; last solve_addr.
     iInstr "Hprog" ; first solve_addr.
 
-    rewrite /shared_buffer. rewrite /map.
-    rewrite /buffer_code1.
+    rewrite /full_buffer /map /buffer_code.
     wp_instr.
-    iInv "Hsecret1_inv" as ">Hsecret1" "Hcls".
-    iDestruct "Hsecret1" as "[Hsecret1 | Hsecret1]".
+    iInv "Hsecret_inv" as ">Hsecret" "Hcls".
+    iDestruct "Hsecret" as "[Hsecret | Hsecret]".
     all: iInstr "Hprog" ; first (subst e_buf ; solve_addr).
-    all: iMod ("Hcls" with "[Hsecret1]") as "_"
+    all: iMod ("Hcls" with "[Hsecret]") as "_"
     ; [ iNext ; iRight ; iAssumption| iModIntro ; wp_pure].
     all: iInstr "Hprog"
     ; [ transitivity (Some b_buf); auto ; solve_addr |].
     all: iInstr "Hprog"
     ; [ transitivity (Some (b_buf ^+ 3)%a); auto ; solve_addr
       | subst e_buf ; solve_addr |].
-    all: iInstr "Hprog" ; iApply "Hφ" ; iFrame.
-    all: iSplitL "Hprog" ; [| iFrame "#"].
-    all: rewrite /codefrag /region_mapsto /buffer_code1.
-    all: replace buffer_code with (finz.seq_between a_first (a_first ^+ 7%nat)%a)
+    all: iInstr "Hprog" ; iApply "Hφ"; iFrame "HPC Hr0 Hr1 # Hdata".
+    all: rewrite /codefrag /region_mapsto /buffer_code.
+    all: replace buffer_codes with (finz.seq_between a_first (a_first ^+ 7%nat)%a)
     ; [iFrame ; auto|].
     all: symmetry
     ; apply region_addrs_of_contiguous_between
@@ -165,96 +129,7 @@ Section shared_buffer.
     ; solve_addr.
   Qed.
 
-
-  Lemma buffer_spec2 (i: CoreN)
-    p b e a a_first a_last
-    (b_buf e_buf: Addr)
-    wadv w1 φ :
-
-    ExecPCPerm p →
-    SubBounds b e a_first a_last ->
-    contiguous_between a a_first a_last →
-    e_buf = (b_buf ^+ (length shared_buffer))%a ->
-    (b_buf ^+ 3 < e_buf)%a →
-    (b_buf ^+ 4 < e_buf)%a →
-
-   ⊢ (( (i, PC) ↦ᵣ WCap p b e a_first
-      ∗ (i, r_t0) ↦ᵣ wadv
-      ∗ (i, r_t1) ↦ᵣ w1
-      ∗ buffer_prog2 a b_buf e_buf
-      ∗ buffer_inv b_buf e_buf
-      ∗ ▷ ((i, PC) ↦ᵣ updatePcPerm wadv
-           ∗ (i, r_t0) ↦ᵣ wadv
-           ∗ (i, r_t1) ↦ᵣ WCap RWX b_buf (b_buf ^+ 3)%a b_buf%a
-           ∗ buffer_prog2 a b_buf e_buf
-           ∗ buffer_inv b_buf e_buf
-           -∗ WP (i, Seq (Instr Executable)) {{ φ }}))
-      -∗ WP (i, Seq (Instr Executable)) {{ φ }})%I.
-  Proof.
-    iIntros (HPCperm HPCbounds Hcont He_buf Hsecret1 Hsecret2)
-      "(HPC & Hr0 & Hr1 & Hprog & #(Hbuffer_pub & Hsecret1_inv & Hsecret2_inv) & Hφ)" .
-    set (e_buf' := e_buf).
-    rename e_buf into eb ; rename e_buf' into e_buf ; subst eb.
-    rewrite {1}/buffer_prog2.
-
-    iDestruct (contiguous_between_program_split with "Hprog") as
-      (buffer_code data a_data) "(Hprog & Hdata & #Hcont1)"
-    ;[apply Hcont|].
-    iDestruct "Hcont1" as %(Hcont_code & Hcont_buffer & Heqapp1 & Ha_data).
-    rewrite /data2.
-    iDestruct (big_sepL2_length with "Hprog") as %Hlength_code.
-    iDestruct (big_sepL2_length with "Hdata") as %Hlength_data.
-    simpl in Hlength_data.
-    inversion Hcont_buffer ; subst ; try discriminate.
-    inversion H0 ; subst ; try discriminate.
-    clear H0.
-    iDestruct ((big_sepL2_singleton (λ _ a_i w_i, (a_i ↦ₐ w_i)%I)) with "Hdata")
-      as "Hdata".
-
-    iAssert (codefrag a_first (buffer_code2 b_buf e_buf)) with "[Hprog]" as "Hprog".
-    { rewrite /codefrag. simpl. rewrite /region_mapsto.
-      simpl in *.
-      replace buffer_code with (finz.seq_between a_first (a_first ^+ 7%nat)%a).
-      done.
-      symmetry.
-      apply region_addrs_of_contiguous_between.
-      replace (a_first ^+ 7%nat)%a with a_data. done.
-      apply contiguous_between_length in Hcont_code.
-      rewrite Hlength_code in Hcont_code.
-      solve_addr. }
-    codefrag_facts "Hprog".
-    iGo "Hprog".
-    replace (a_first ^+ 7)%a with a_data ; last solve_addr.
-    iInstr "Hprog" ; first solve_addr.
-
-    rewrite /shared_buffer. rewrite /map.
-    rewrite /buffer_code2.
-    wp_instr.
-    iInv "Hsecret2_inv" as ">Hsecret2" "Hcls".
-    iDestruct "Hsecret2" as "[Hsecret2 | Hsecret2]".
-    all: iInstr "Hprog" ; first (subst e_buf ; solve_addr).
-    all: iMod ("Hcls" with "[Hsecret2]") as "_"
-    ; [ iNext ; iRight ; iAssumption| iModIntro ; wp_pure].
-    all: iInstr "Hprog"
-    ; [ transitivity (Some b_buf); auto ; solve_addr |].
-    all: iInstr "Hprog"
-    ; [ transitivity (Some (b_buf ^+ 3)%a); auto ; solve_addr
-      | subst e_buf ; solve_addr |].
-    all: iInstr "Hprog" ; iApply "Hφ" ; iFrame.
-    all: iSplitL "Hprog" ; [| iFrame "#"].
-    all: rewrite /codefrag /region_mapsto /buffer_code1.
-    all: replace buffer_code with (finz.seq_between a_first (a_first ^+ 7%nat)%a)
-    ; [iFrame ; auto|].
-    all: symmetry
-    ; apply region_addrs_of_contiguous_between
-    ; replace (a_first ^+ 7%nat)%a with a_data ; [done|].
-    all: apply contiguous_between_length in Hcont_code
-    ; rewrite Hlength_code in Hcont_code
-    ; solve_addr.
-  Qed.
-
-
-  Lemma buffer_full_run_spec1
+  Lemma buffer_full_run_spec
     (i: CoreN)
     p b e a a_first a_last (* PC capabilities *)
     (b_buf e_buf: Addr) (* Shared buffer *)
@@ -264,8 +139,8 @@ Section shared_buffer.
     ExecPCPerm p →
     SubBounds b e a_first a_last ->
     contiguous_between a a_first a_last →
-    e_buf = (b_buf ^+ (length shared_buffer))%a ->
-    (b_buf + 5)%a = Some (b_buf ^+ 5)%a →
+    e_buf = (b_buf ^+ (length full_buffer))%a ->
+    (b_buf + (length full_buffer))%a = Some (b_buf ^+ (length full_buffer))%a →
 
     Forall (λ w, is_cap w = false) adv →
     (b_adv + length adv)%a = Some e_adv →
@@ -277,8 +152,9 @@ Section shared_buffer.
          ∗ (i, r_t0) ↦ᵣ WCap RWX b_adv e_adv b_adv
          ∗ ([∗ map] r↦w ∈ rmap, r ↦ᵣ w ∗ ⌜is_cap w = false⌝)
 
-         ∗ buffer_prog1 a b_buf e_buf
+         ∗ buffer_prog a b_buf e_buf
          ∗ ([∗ map] a↦w ∈ mkregion b_adv e_adv adv, a ↦ₐ w)
+         ∗ ([∗ map] a↦w ∈ mkregion b_buf (b_buf ^+3)%a public_buffer, a ↦ₐ w)
          ∗ buffer_inv b_buf e_buf
 
          -∗ WP (i, Seq (Instr Executable)) {{ λ _, True }})%I.
@@ -286,100 +162,19 @@ Section shared_buffer.
   Proof.
     iIntros (HPCperm HPCbounds Hcont He_buf HV_buf
                HVadv Hlength_adv Hrmap_dom)
-      "(HPC & Hr0 & Hrmap & Hprog & Hadv & #(Hbuffer_pub & Hsecret1_inv & Hsecret2_inv))" .
+      "(HPC & Hr0 & Hrmap & Hprog & Hadv & Hbuffer_pub & #Hsecret_inv)" .
 
     (* Continuation - executes completelety after the jump to the adversary *)
     iDestruct (mkregion_sepM_to_sepL2 with "Hadv") as "Hadv". done.
     iDestruct (region_integers_alloc' _ _ _ b_adv _ RWX with "Hadv") as ">#Hadv". done.
     iDestruct (jmp_to_unknown with "Hadv") as "#Hcont".
 
-    (* Extract the register r1 *)
-    assert (is_Some (rmap !! (i,r_t1)))
-      as [w1 Hw1]
-           by (rewrite elem_of_gmap_dom Hrmap_dom; set_solver+). 
-      iDestruct (big_sepM_delete _ _ (i, r_t1) with "Hrmap") as "[[Hr1 %HVw1] Hrmap]"
-      ; first eauto.
-
-    iApply (buffer_spec1 with "[-]"); eauto ; try solve_addr.
-    iFrame "∗#".
-    iNext. iIntros "(HPC & Hr0 & Hr1 & _)".
-
-    (* Show that the contents of r1 is safe *)
-    iAssert ( interp (WCap RWX b_buf (b_buf ^+ 3 )%a b_buf)) as "HvR1".
-    { rewrite (fixpoint_interp1_eq (WCap _ b_buf _ _)).
-      cbn.
-      iApply (big_sepL_mono with "Hbuffer_pub").
-      cbn.
-      intros.
-      iIntros "#Hinv".
-      iExists _.
-      iFrame "#".
-      iSplit; do 2 iModIntro ; iIntros (?) "?" ; iAssumption.
-    }
-
-    (* Show that the contents of unused registers is safe *)
-    set (rmap' := delete (i, r_t1) rmap).
-    iAssert ([∗ map] r↦w ∈ rmap', r ↦ᵣ w ∗ interp w)%I with "[Hrmap]" as "Hrmap".
-    { iApply (big_sepM_mono with "Hrmap"). intros r w Hr'. cbn. iIntros "[? %Hw]". iFrame.
-      destruct w; [| by inversion Hw]. rewrite fixpoint_interp1_eq //. }
-
-    (* put the other registers back into the register map *)
-    iDestruct (big_sepM_insert _ _ (i, r_t1) with "[$Hrmap Hr1]") as "Hrmap".
-    { apply not_elem_of_dom ; set_solver+. }
-    iFrame "∗#".
-    subst rmap' ; rewrite insert_delete.
-    iDestruct (big_sepM_insert _ _ (i, r_t0) with "[$Hrmap Hr0]") as "Hrmap".
-    { rewrite lookup_insert_ne ; [| clear Hrmap_dom ; simplify_pair_eq].
-    apply not_elem_of_dom . rewrite Hrmap_dom; set_solver+. }
-    by iFrame.
-    iApply (wp_wand with "[-]").
-    { iApply "Hcont"; cycle 1. iFrame. iPureIntro. rewrite !dom_insert_L Hrmap_dom.
-      clear Hrmap_dom.
-      do 2 rewrite singleton_union_difference_L.
-      set_solver+. }
-    eauto.
-  Qed.
-  
-  Lemma buffer_full_run_spec2
-    (i: CoreN)
-    p b e a a_first a_last (* PC capabilities *)
-    (b_buf e_buf: Addr) (* Shared buffer *)
-    b_adv e_adv adv (* Adversary *)
-    rmap :
-
-    ExecPCPerm p →
-    SubBounds b e a_first a_last ->
-    contiguous_between a a_first a_last →
-    e_buf = (b_buf ^+ (length shared_buffer))%a ->
-    (b_buf + 5)%a = Some (b_buf ^+ 5)%a →
-
-    Forall (λ w, is_cap w = false) adv →
-    (b_adv + length adv)%a = Some e_adv →
-
-
-    dom (gset (CoreN*RegName)) rmap =
-      (set_map (fun r => (i,r)) all_registers_s) ∖ {[ (i, PC); (i, r_t0) ]} →
-
-    ⊢ (  (i, PC) ↦ᵣ WCap p b e a_first
-         ∗ (i, r_t0) ↦ᵣ WCap RWX b_adv e_adv b_adv
-         ∗ ([∗ map] r↦w ∈ rmap, r ↦ᵣ w ∗ ⌜is_cap w = false⌝)
-
-         ∗ buffer_prog2 a b_buf e_buf
-         ∗ ([∗ map] a↦w ∈ mkregion b_adv e_adv adv, a ↦ₐ w)
-         ∗ buffer_inv b_buf e_buf
-
-         -∗ WP (i, Seq (Instr Executable)) {{ λ _, True }})%I.
-
-  Proof.
-    iIntros (HPCperm HPCbounds Hcont He_buf HV_buf
-               HVadv Hlength_adv Hrmap_dom)
-      "(HPC & Hr0 & Hrmap & Hprog & Hadv & #(Hbuffer_pub & Hsecret1_inv & Hsecret2_inv))" .
-
-    (* Continuation - executes completelety after the jump to the adversary *)
-    iDestruct (mkregion_sepM_to_sepL2 with "Hadv") as "Hadv". done.
-    iDestruct (region_integers_alloc' _ _ _ b_adv _ RWX with "Hadv") as ">#Hadv". done.
-    iDestruct (jmp_to_unknown with "Hadv") as "#Hcont".
-
+    iDestruct ( mkregion_sepM_to_sepL2 with "Hbuffer_pub") as "Hbuffer_pub"
+    ; first solve_addr.
+    iDestruct (region_integers_alloc' _ _ _ b_buf _ RWX with "Hbuffer_pub") as
+      ">#Hbuffer_public".
+    rewrite /public_buffer ; cbn.
+    repeat (apply Forall_cons_2 ; auto).
     (* Extract the register r1 *)
     assert (is_Some (rmap !! (i,r_t1)))
       as [w1 Hw1]
@@ -387,21 +182,9 @@ Section shared_buffer.
       iDestruct (big_sepM_delete _ _ (i, r_t1) with "Hrmap") as "[[Hr1 %HVw1] Hrmap]"
       ; first eauto.
 
-    iApply (buffer_spec2 with "[-]"); eauto ; try solve_addr. iFrame "∗#".
+    iApply (buffer_spec with "[-]"); eauto ; try solve_addr.
+    iFrame "∗#".
     iNext. iIntros "(HPC & Hr0 & Hr1 & _)".
-
-    (* Show that the contents of r1 is safe *)
-    iAssert ( interp (WCap RWX b_buf (b_buf ^+ 3 )%a b_buf)) as "HvR1".
-    { rewrite (fixpoint_interp1_eq (WCap _ b_buf _ _)).
-      cbn.
-      iApply (big_sepL_mono with "Hbuffer_pub").
-      cbn.
-      intros.
-      iIntros "#Hinv".
-      iExists _.
-      iFrame "#".
-      iSplit; do 2 iModIntro ; iIntros (?) "?" ; iAssumption.
-    }
 
     (* Show that the contents of unused registers is safe *)
     set (rmap' := delete (i, r_t1) rmap).
@@ -426,7 +209,98 @@ Section shared_buffer.
     eauto.
   Qed.
 
-End shared_buffer.
+
+  Lemma interp_updatePcPerm_adv p b e a :
+    p = RX \/ p = RWX ->
+    ⊢ interp (WCap p b e a) -∗ (∀ i r, interp_expression i r (updatePcPerm (WCap p b e a))).
+  Proof.
+    iIntros (Hp) "#Hw".
+    iIntros (rmap i). destruct Hp as [ -> | -> ] ; iApply fundamental ; eauto.
+  Qed.
+
+
+  Lemma jmp_to_unknown_adv p b e a :
+    p = RX \/ p = RWX ->
+    ⊢ interp (WCap p b e a) -∗
+      ∀ (i: CoreN) rmap,
+          ⌜dom (gset (CoreN*RegName)) rmap = (set_map (fun r=> (i,r)) all_registers_s) ∖ {[ (i, PC) ]}⌝ →
+          (i, PC) ↦ᵣ updatePcPerm (WCap p b e a)
+          ∗ ([∗ map] r↦w ∈ rmap, r ↦ᵣ w ∗ interp w)
+          -∗ WP (i, Seq (Instr Executable)) {{ λ v, ⌜v = (i, HaltedV)⌝ →
+               ∃ r : Reg, full_map r i ∧ registers_mapsto r }}.
+  Proof.
+    iIntros (Hp) "#Hw". iDestruct (interp_updatePcPerm_adv with "Hw") as "Hw'"
+    ; eauto.
+    iIntros (i rmap Hrmap).
+    set rmap' := <[ (i, PC) := (WInt 0%Z: Word) ]> rmap
+        : gmap (CoreN*RegName) Word.
+    iSpecialize ("Hw'" $! rmap').
+    iIntros "(HPC & Hr)". unfold interp_expression, interp_expr, interp_conf. cbn.
+    iApply "Hw'". iClear "Hw'". iFrame. rewrite /registers_mapsto.
+    iDestruct (big_sepM_sep with "Hr") as "(Hr & HrV)".
+    iSplitL "HrV"; [iSplit|].
+    { unfold full_map. iIntros (r).
+      destruct (decide (r = PC)).
+      { subst r. rewrite lookup_insert. iPureIntro. eauto. }
+      rewrite lookup_insert_ne;[| clear Hrmap; simplify_pair_eq].
+      iPureIntro. rewrite elem_of_gmap_dom Hrmap.
+      clear Hrmap; set_solver. }
+    { iIntros (j ri v Hri Hvs).
+      rewrite lookup_insert_ne in Hvs;[| clear Hrmap; simplify_pair_eq].
+      iDestruct (big_sepM_lookup _ _ (j, ri) with "HrV") as "HrV"; eauto.
+    }
+    rewrite insert_insert. iApply big_sepM_insert.
+    { apply elem_of_gmap_dom_none. rewrite Hrmap ; clear Hrmap.
+      set_solver. }
+    iFrame.
+  Qed.
+
+  Lemma adversary_full_run_spec
+    (i: CoreN)
+    (Adv : adv_prog)
+    (b_buf e_buf: Addr) (* Shared buffer *)
+    rmap :
+
+    let b_adv := (adv_start Adv) in
+    let e_adv := (adv_end Adv) in
+    let adv := (adv_instrs Adv) in
+    let l_buf := (length full_buffer) in
+
+    e_buf = (b_buf ^+ l_buf )%a ->
+    (b_buf + l_buf)%a = Some (b_buf ^+ l_buf)%a →
+
+    dom (gset (CoreN*RegName)) rmap =
+      (set_map (fun r => (i,r)) all_registers_s) ∖ {[ (i, PC)]} →
+
+    ⊢ (  (i, PC) ↦ᵣ WCap RWX b_adv e_adv b_adv
+         ∗ ([∗ map] r↦w ∈ rmap, r ↦ᵣ w ∗ ⌜is_cap w = false⌝)
+         ∗ ([∗ map] a↦w ∈ adv_region Adv, a ↦ₐ w)
+         ∗ buffer_inv b_buf e_buf
+
+         -∗ WP (i, Seq (Instr Executable)) {{ λ _, True }})%I.
+  Proof.
+    intros b_adv e_adv adv l_buf.
+    iIntros (He_buf HV_buf Hrmap_dom)
+      "(HPC & Hrmap & Hadv & #Hsecret_inv)" .
+    subst.
+    (* Continuation - executes completelety after the jump to the adversary *)
+    iDestruct (mkregion_sepM_to_sepL2 with "Hadv") as "Hadv".
+    { pose proof (adv_size Adv); solve_addr. }
+    iDestruct (region_integers_alloc' with "Hadv") as ">#Hadv"
+    ; first apply (adv_valid Adv).
+    iDestruct (jmp_to_unknown_adv with "Hadv") as "#Hcont"; first by right.
+
+    iAssert ([∗ map] r↦w ∈ rmap, r ↦ᵣ w ∗ interp w)%I with "[Hrmap]" as "Hrmap".
+    { iApply (big_sepM_mono with "Hrmap"). intros r w Hr'. cbn. iIntros "[? %Hw]". iFrame.
+      destruct w; [| by inversion Hw]. rewrite fixpoint_interp1_eq //. }
+
+    iApply (wp_wand with "[-]").
+    { iApply "Hcont"; cycle 1. iFrame. iPureIntro. assumption. }
+    eauto.
+  Qed.
+
+
+End buffer.
 
 Section adequacy.
 
@@ -436,43 +310,43 @@ Section adequacy.
   Context {reg_preg: gen_heapPreG (CoreN * RegName) Word Σ}.
   Context `{MP: MachineParameters}.
 
+
   (** Shared buffer adequacy theorem *)
-  Definition mem_inv (m : Mem) (b_buf : Addr):=
-    (m !! (b_buf^+3)%a = Some (WInt 0) \/ m !! (b_buf^+3)%a = Some (WInt 42))
-    /\ (m !! (b_buf^+4)%a = Some (WInt 0) \/ m !! (b_buf^+4)%a = Some (WInt (-42))).
+
+
+  Definition mem_inv (m : Mem) (b_buf : Addr ):=
+    (m !! (b_buf^+3)%a = Some (WInt 0) \/ m !! (b_buf^+3)%a = Some (WInt 42) ).
 
   Ltac solve_addr' SB Hsbuf b_buf e_buf :=
     ( pose proof (Hsize := prog_size SB)
       ; rewrite Hsbuf in Hsize
-      ; subst b_buf e_buf ; solve_addr) .
+      ; subst b_buf e_buf ; solve_addr).
 
   Lemma adequacy_shared_buffer
     (m m': Mem) (reg reg': Reg) (es : list cap_lang.expr)
-    (P1 Adv1 P2 Adv2 : prog) (* Programs and adversary *)
-    (SB : prog) (* shared buffer *)
+    (P Adv1 B : prog) (* Programs, adversaries and buffer *)
+    (Adv2 : adv_prog)
     (i j : CoreN) :
 
-    let b_buf := (prog_start SB) in
-    let e_buf := (prog_end SB) in
+    let b_buf := (prog_start B) in
+    let e_buf := (prog_end B) in
 
     (* Machine with 2 cores identified by {0, 1} *)
     machine_base.CoreNum = 2 ->
     i = core_zero ->
     j = (i^+1)%f ->
-    
+
     (* The adversary contains only instructions *)
     Forall (λ w, is_cap w = false) (prog_instrs Adv1) →
-    Forall (λ w, is_cap w = false) (prog_instrs Adv2) →
-    (* The programs P1 and P2 are the instructions of buffer_codeX *)
-    prog_instrs P1 = (buffer_code1 b_buf e_buf ++ data1 b_buf e_buf) ->
-    prog_instrs P2 = (buffer_code2 b_buf e_buf ++ data2 b_buf e_buf) ->
-    (* The initial content of the shared buffer *)
-    prog_instrs SB = shared_buffer ->
+    (* The program P contains the instructions of buffer_code *)
+    prog_instrs P = (buffer_code b_buf e_buf ++ data b_buf e_buf) ->
+    (* The initial content of the full buffer *)
+    prog_instrs B = full_buffer ->
 
     (* Initial state *)
-    is_initial_registers_with_adv P1 Adv1 r_t0 reg i ->
-    is_initial_registers_with_adv P2 Adv2 r_t0 reg j ->
-    is_initial_memory [P1;P2;Adv1;Adv2;SB] [] m ->
+    is_initial_registers_with_adv P Adv1 r_t0 reg i ->
+    is_initial_registers_adv Adv2 reg j ->
+    is_initial_memory [P;Adv1;B] [Adv2] m ->
 
     (* The invariant holds on the initial memory *)
     mem_inv m b_buf ->
@@ -483,7 +357,7 @@ Section adequacy.
 
   Proof.
     intros b_buf e_buf.
-    intros Hn_cores Hi Hj Hadv1 Hadv2 Hprog1 Hprog2 Hsbuf Hreg1 Hreg2 Hmem Hmem_inv Hstep.
+    intros Hn_cores Hi Hj Hadv1 Hprog Hsbuf Hreg1 Hreg2 Hmem Hmem_inv Hstep.
     apply erased_steps_nsteps in Hstep as (n & κs & Hstep).
 
     (* We apply the Iris adequacy theorem, and we unfold the definition,
@@ -507,15 +381,7 @@ Section adequacy.
     (* Split the memory into 5 parts: prog1, prog2, adv1, adv2, shared_buffer*)
     iDestruct (big_sepM_subseteq with "Hmem") as "Hmem".
     by apply Hmem.
-    iDestruct (big_sepM_union with "Hmem") as "[Hprog1 Hmem]".
-    { rewrite /is_initial_memory in Hmem.
-      destruct Hmem as (_ & Hmem)
-      ; rewrite /disjoint_list_map /= in Hmem
-      ; destruct Hmem as (?&?&?&?&?).
-      repeat (apply map_disjoint_union_l_2 ; auto)
-      ; auto.
-    }
-    iDestruct (big_sepM_union with "Hmem") as "[Hprog2 Hmem]".
+    iDestruct (big_sepM_union with "Hmem") as "[Hprog Hmem]".
     { rewrite /is_initial_memory in Hmem.
       destruct Hmem as (_ & Hmem)
       ; rewrite /disjoint_list_map /= in Hmem
@@ -531,7 +397,7 @@ Section adequacy.
       repeat (apply map_disjoint_union_l_2 ; auto)
       ; auto.
     }
-    iDestruct (big_sepM_union with "Hmem") as "[Hadv2 Hmem]".
+    iDestruct (big_sepM_union with "Hmem") as "[Hbuffer Hmem]".
     { rewrite /is_initial_memory in Hmem.
       destruct Hmem as (_ & Hmem)
       ; rewrite /disjoint_list_map /= in Hmem
@@ -539,66 +405,47 @@ Section adequacy.
       repeat (apply map_disjoint_union_l_2 ; auto)
       ; auto.
     }
-    iDestruct (big_sepM_union with "Hmem") as "[Hbuffer _]"
+    iDestruct (big_sepM_union with "Hmem") as "[Hadv2 _]"
     ; first apply map_disjoint_empty_r.
 
 
 
     (* Allocation of all the required invariants *)
     (* Split the shared_buffer into public and secret buffer *)
-    rewrite /buffer_inv.
-    iDestruct (mkregion_sepM_to_sepL2 with "Hbuffer") as "Hbuffer".
-    apply (prog_size SB).
-    rewrite Hsbuf /shared_buffer.
-    rewrite ( finz_seq_between_split b_buf (b_buf ^+3)%a e_buf ).
-    2: solve_addr' SB Hsbuf b_buf e_buf.
-    iDestruct (big_sepL2_app' _ _ _ _
-                 (finz.seq_between b_buf (b_buf ^+ 3)%a)
-                 (finz.seq_between (b_buf ^+ 3)%a e_buf)
-                 public_buffer secret_buffer
-                with "Hbuffer") as "[Hpublic Hsecret]".
-    { cbn. rewrite finz_seq_between_length. apply finz_incr_iff_dist.
-     solve_addr' SB Hsbuf b_buf e_buf. }
+    rewrite {3}/prog_region Hsbuf /full_buffer.
+    rewrite mkregion_app.
+    2:{ solve_addr' B Hsbuf b_buf e_buf. }
+    iDestruct (big_sepM_union with "Hbuffer") as "[Hpublic Hsecret]".
+    {
+    rewrite /mkregion ; cbn.
+    do 3 (rewrite finz_seq_between_cons ; [| solve_addr' B Hsbuf b_buf e_buf ]).
+    rewrite finz_seq_between_empty  ; [| solve_addr' B Hsbuf b_buf e_buf ].
+    rewrite finz_seq_between_cons ; [| solve_addr' B Hsbuf b_buf e_buf ].
+    rewrite finz_seq_between_empty  ; [| solve_addr' B Hsbuf b_buf e_buf ].
+    cbn.
+    apply map_disjoint_insert_r_2 ; [|apply map_disjoint_empty_r ].
+    assert ( (prog_start B) ≠  (prog_start B ^+ 3%nat)%a )
+      by solve_addr' B Hsbuf b_buf e_buf.
+    assert ( (prog_start B ^+ 1%nat)%a ≠  (prog_start B ^+ 3%nat)%a )
+      by solve_addr' B Hsbuf b_buf e_buf.
+    assert ( ((prog_start B ^+ 1) ^+ 1)%a ≠  (prog_start B ^+ 3%nat)%a )
+      by solve_addr' B Hsbuf b_buf e_buf.
+    simplify_map_eq ; reflexivity.
+    }
+    iDestruct (mkregion_sepM_to_sepL2 with "Hsecret") as "Hsecret".
+    solve_addr' B Hsbuf b_buf e_buf.
     (* Allocates the invariant about the secret buffer *)
     rewrite /secret_buffer ; simpl.
-    rewrite (finz_seq_between_cons (b_buf ^+ 3)%a).
-    2: { solve_addr' SB Hsbuf b_buf e_buf. }
-    replace ( ((b_buf ^+ 3) ^+ 1)%a ) with ( (b_buf ^+ 4)%a ) by solve_addr.
-    replace (finz.seq_between (b_buf ^+ 4)%a e_buf)
-      with ([(b_buf ^+ 4)%a]).
+    replace (finz.seq_between (prog_start B ^+ 3%nat)%a (prog_end B))
+      with ([(prog_start B ^+ 3%nat)%a]).
     2: { rewrite finz_seq_between_singleton
-         ; [done| solve_addr' SB Hsbuf b_buf e_buf]. }
-    simpl.
-    iDestruct "Hsecret" as "(Hsecret1 & Hsecret2& _)".
+         ; [done| solve_addr' B Hsbuf b_buf e_buf]. }
+    simpl. iDestruct "Hsecret" as "[Hsecret _]".
     iMod (inv_alloc (invG0 := Hinv)
             (Nsb.@(b_buf ^+ 3)%a)
             ⊤ ((b_buf ^+ 3)%a ↦ₐ WInt 0 ∨ (b_buf ^+ 3)%a ↦ₐ WInt 42)
-           with "[Hsecret1]") as "#Hinv_secret1".
+           with "[Hsecret]") as "#Hinv_secret".
     { iNext ; iLeft ; iFrame. }
-    iMod (inv_alloc (Nsb.@(b_buf ^+ 4)%a)
-            ⊤ ((b_buf ^+ 4)%a ↦ₐ WInt 0 ∨ (b_buf ^+ 4)%a ↦ₐ WInt (-42))
-           with "[Hsecret2]") as "#Hinv_secret2".
-    { iNext ; iLeft ; iFrame. }
-
-    (* Allocates the invariant about the public buffer *)
-      assert (Hpublic_int : Forall (fun w => is_cap w = false) public_buffer).
-      {  rewrite /public_buffer /= ; auto.
-      }
-
-    iDestruct (big_sepL2_mono _ (fun _ a w => (a ↦ₐ w ∗ interp w)%I) with "Hpublic")
-      as "Hpublic".
-    { intros ? ? ? ? Hsome ; cbn. iIntros ; iFrame.
-      eapply Forall_lookup_1 in Hsome ; eauto ; cbn in Hsome.
-      destruct y2; [iApply interp_int| by cbn in Hsome].
-    }
-    iDestruct (region_inv_alloc with "[$Hpublic]") as ">#Hpublic".
-    iDestruct ( big_sepL2_to_big_sepL_l with "Hpublic") as "Hinv_public".
-    { cbn.
-      rewrite finz_seq_between_length.
-      do 3 (rewrite finz_dist_S ; last solve_addr' SB Hsbuf b_buf e_buf).
-      by rewrite finz_dist_0 ; last  solve_addr' SB Hsbuf b_buf e_buf.
-    }
-    iClear "Hpublic".
 
     iModIntro.
     iSplitL.
@@ -621,7 +468,7 @@ Section adequacy.
        *)
       rewrite /is_initial_registers in Hreg1, Hreg2.
       destruct Hreg1 as ((Hreg1_some & Hreg1_dom & Hreg1_valid) & Hreg1_adv & Hneq1).
-      destruct Hreg2 as ((Hreg2_some & Hreg2_dom & Hreg2_valid) & Hreg2_adv & Hneq2).
+      destruct Hreg2 as (Hreg2_some & Hreg2_dom & Hreg2_valid).
       set (rmap_i := @set_map _ _ _ _ _ _ _
                        (@gset_union (CoreN * RegName) _ _)
                        (fun r : RegName => (i,r)) all_registers_s).
@@ -697,7 +544,7 @@ Section adequacy.
 
       (* For each core, we prove the WP, using the specification previously
          defined *)
-      iSplitL "Hprog1 Hadv1 Hreg_i".
+      iSplitL "Hprog Hadv1 Hreg_i Hpublic".
       - (* We extracts the needed registers for the full_run_spec *)
       iDestruct (big_sepM_delete _ _ (i, PC) with "Hreg_i") as "[HPC_i Hreg_i]".
       apply map_filter_lookup_Some_2 ; [|by subst Pi ; cbn] ; eauto.
@@ -706,11 +553,12 @@ Section adequacy.
       apply map_filter_lookup_Some_2 ; [|by subst Pi ; cbn] ; eauto.
 
       (* Apply the specification *)
-      iApply (buffer_full_run_spec1 _ _ _ _ _  _ (prog_end P1) _ _ _ _ _
-               with "[$HPC_i $Hadv_i Hreg_i Hprog1 Hadv1]") ; cycle -1.
-      iDestruct (mkregion_sepM_to_sepL2 with "Hprog1") as "Hprog1".
-      { apply (prog_size P1). }
-      rewrite /buffer_prog1 Hprog1.
+      iApply (buffer_full_run_spec _ _ _ _ _  _ (prog_end P) _ _ _ _ _
+               with "[$HPC_i $Hadv_i Hreg_i Hprog Hadv1 Hpublic]") ; cycle -1.
+      iDestruct (mkregion_sepM_to_sepL2 with "Hprog") as "Hprog".
+      { apply (prog_size P). }
+
+      rewrite /buffer_prog Hprog.
       iFrame "#∗".
 
       iAssert ([∗ map] r↦w ∈
@@ -738,11 +586,11 @@ Section adequacy.
       apply ExecPCPerm_RWX.
       { split ; [solve_addr |].
         split ; [|solve_addr ].
-        pose proof (prog_size P1) ; solve_addr. }
+        pose proof (prog_size P) ; solve_addr. }
       { apply contiguous_between_region_addrs.
-        pose proof (prog_size P1) ; solve_addr. }
-      { solve_addr' SB Hsbuf b_buf e_buf. }
-      { solve_addr' SB Hsbuf b_buf e_buf. }
+        pose proof (prog_size P) ; solve_addr. }
+      { solve_addr' B Hsbuf b_buf e_buf. }
+      { solve_addr' B Hsbuf b_buf e_buf. }
       assumption.
       apply (prog_size Adv1).
       { rewrite !dom_delete_L.
@@ -760,92 +608,61 @@ Section adequacy.
           apply map_filter_lookup_Some_2 ; [eauto| cbn ; by apply not_eq_sym].
         }
         by subst Pj ; cbn.
-        iDestruct (big_sepM_delete _ _ (j, r_t0) with "Hreg_j") as "[Hadv_j Hreg_j]".
-        rewrite lookup_delete_ne ; [|simplify_pair_eq] ; eauto.
-        apply map_filter_lookup_Some_2.
-        { subst regs_ni Pj Pi ; cbn.
-          apply map_filter_lookup_Some_2 ; [eauto| cbn ; by apply not_eq_sym].
-        }
-        by subst Pj ; cbn.
-
-        iApply (buffer_full_run_spec2 _ _ _ _ _  _ (prog_end P2) _ _ _ _ _
-                 with "[$HPC_j $Hadv_j Hreg_j Hprog2 Hadv2]") ; cycle -1.
-        iDestruct (mkregion_sepM_to_sepL2 with "Hprog2") as "Hprog2".
-        { apply (prog_size P2). }
-        rewrite /buffer_prog2 Hprog2.
-        iFrame "#∗".
-
-        iAssert ([∗ map] r↦w ∈
-                   (delete (j, r_t0) (delete (j, PC) (filter Pj regs_ni)) )
-                  , r ↦ᵣ w ∗ ⌜is_cap w = false⌝)%I
-          with "[Hreg_j]" as "Hreg_j".
-        { iApply (big_sepM_mono with "Hreg_j"). intros r w Hr. cbn.
-          apply lookup_delete_Some in Hr as [Hr_r0 Hr].
-          apply lookup_delete_Some in Hr as [Hr_PC Hr].
-          assert (Hr' := Hr).
-          apply (map_filter_lookup_Some_1_2
-                   (λ v : CoreN * RegName * Word, Pj v) regs_ni r w) in Hr.
-          subst Pj ; cbn in Hr.
-          destruct r as [? r] ; inversion Hr ; subst.
-          feed pose proof (Hreg2_valid r) as HH. clear -Hr_PC ; set_solver.
-          destruct HH as [? (Hr_reg & Hcap)].
-          iIntros ; iFrame ; iPureIntro.
-          clear -Hr_reg Hr' Hcap.
-          cbn in *.
-          apply map_filter_lookup_Some in Hr'.
-          destruct Hr' as [? _].
-          subst regs_ni.
-          apply map_filter_lookup_Some_1_1 in H.
-          simplify_map_eq. auto.
-        }
-        iFrame.
-        apply ExecPCPerm_RWX.
-        { split ; [solve_addr |].
-          split ; [|solve_addr ].
-          pose proof (prog_size P2) ; solve_addr. }
-        { apply contiguous_between_region_addrs.
-          pose proof (prog_size P2) ; solve_addr. }
-        { solve_addr' SB Hsbuf b_buf e_buf. }
-        { solve_addr' SB Hsbuf b_buf e_buf. }
-        assumption.
-        apply (prog_size Adv2).
+        iApply (adversary_full_run_spec j _ b_buf e_buf (delete (j, PC) (filter Pj regs_ni))
+                 with "[$HPC_j Hreg_j $Hadv2]").
+        solve_addr' B Hsbuf b_buf e_buf.
+        solve_addr' B Hsbuf b_buf e_buf.
         { rewrite !dom_delete_L.
           set (X := set_map (λ r : RegName, (j, r)) all_registers_s).
-          rewrite - !difference_difference_L.
           replace ( dom (gset (CoreN * RegName)) (filter Pj regs_ni)) with X by set_solver.
           set_solver.
         }
+        iFrame "#".
+
+        iAssert ([∗ map] r↦w ∈
+                   delete (j, PC) (filter Pj regs_ni)
+                  , r ↦ᵣ w ∗ ⌜is_cap w = false⌝)%I
+          with "[Hreg_j]" as "Hreg_j".
+        { iApply (big_sepM_mono with "Hreg_j"). intros r w Hr. cbn.
+          apply lookup_delete_Some in Hr as [Hr_PC Hr].
+          assert (Hr' := Hr).
+          apply (map_filter_lookup_Some_1_2 Pj regs_ni r w) in Hr.
+          do 2 (apply map_filter_lookup_Some_1_1 in Hr').
+          subst Pj ; cbn in Hr.
+
+          destruct r as [? r] ; inversion Hr ; subst.
+          feed pose proof (Hreg2_valid r) as HH. clear -Hr_PC ; set_solver.
+          destruct HH as [? (Hr_reg & Hcap)].
+          clear -Hr_reg Hr' Hcap.
+          iIntros ; iFrame ; iPureIntro.
+          cbn in *.
+          simplify_map_eq. auto.
+        }
+        iFrame.
     }
 
     (** The invariant holds on the resulting memory *)
     iIntros (es' t2) "%Hes %Hlength_es %Hstuck [Hreg' Hmem'] Hopt _".
     rewrite /mem_inv.
-    iInv "Hinv_secret1" as ">Hsecret1" "_".
-    iInv "Hinv_secret2" as ">Hsecret2" "_".
-    assert (Hneq: (b_buf ^+ 4)%a ≠ (b_buf ^+ 3)%a )
-             by solve_addr' SB Hsbuf b_buf e_buf.
-    solve_ndisj ; clear Hneq.
-    iDestruct "Hsecret1" as "[Hsecret1 | Hsecret1 ]"
-    ; iDestruct "Hsecret2" as "[Hsecret2 | Hsecret2 ]"
-    ; iDestruct (gen_heap_valid m' with "Hmem' Hsecret1") as "#%secret1"
-    ; iDestruct (gen_heap_valid m' with "Hmem' Hsecret2") as "#%secret2"
+    iInv "Hinv_secret" as ">Hsecret" "_".
+    iDestruct "Hsecret" as "[Hsecret | Hsecret ]"
+    ; iDestruct (gen_heap_valid m' with "Hmem' Hsecret") as "#%secret"
     ; (iApply fupd_mask_intro_discard ; [set_solver|iPureIntro])
-    ; split
-    ; [ left | left | left | right | right | left | right | right]
+    ; [ left | right]
     ; assumption.
 
-      Unshelve.
-      apply gmap_fmap.
-      apply gmap_omap.
-      apply gmap_merge.
-      solve_decision.
-      apply gset_empty.
-      apply gset_singleton.
-      apply gset_union.
-      apply gset_intersection.
-      apply gset_difference.
-      apply gset_dom_spec.
-      apply gset_leibniz.
+    Unshelve.
+    apply gmap_fmap.
+    apply gmap_omap.
+    apply gmap_merge.
+    solve_decision.
+    apply gset_empty.
+    apply gset_singleton.
+    apply gset_union.
+    apply gset_intersection.
+    apply gset_difference.
+    apply gset_dom_spec.
+    apply gset_leibniz.
   Qed.
 
 End adequacy.
