theories/examples/template_adequacy_concurrency.v
@@ -8,6 +8,7 @@ From cap_machine Require Import
 From cap_machine.examples Require Import addr_reg_sample.
 From cap_machine.examples Require Export mkregion_helpers disjoint_regions_tactics.
 
+(* TODO simplify prog and adv_prog, it should be only one record *)
 Record prog := MkProg {
   prog_start: Addr;
   prog_end: Addr;
@@ -20,6 +21,33 @@ Record prog := MkProg {
 Definition prog_region (P: prog): gmap Addr Word :=
   mkregion (prog_start P) (prog_end P) (prog_instrs P).
 
+Definition can_address_only (w: Word) (addrs: gset Addr): Prop :=
+  match w with
+  | WInt _ => True
+  | WCap _ b e _ =>
+      forall a, (b <= a < e)%a -> a ∈ addrs
+end.
+
+Record adv_prog :=
+  MkAdvProg {
+      adv_start: Addr;
+      adv_end: Addr;
+      adv_instrs: list Word;
+
+      adv_size:
+      (adv_start + length adv_instrs)%a = Some adv_end;
+      adv_valid:
+      Forall (fun w => is_cap w = false) adv_instrs;
+      (* TODO relax the property into the following one *)
+      (* Forall *)
+      (*   (fun w => can_address_only w *)
+      (*            (dom _ (mkregion adv_start adv_end adv_instrs))) *)
+      (*   adv_instrs; *)
+    }.
+
+Definition adv_region (P: adv_prog): gmap Addr Word :=
+  mkregion (adv_start P) (adv_end P) (adv_instrs P).
+
 Lemma prog_region_dom (P: prog):
   dom (gset Addr) (prog_region P) =
   list_to_set (finz.seq_between (prog_start P) (prog_end P)).
@@ -28,7 +56,6 @@ Proof.
   rewrite finz_seq_between_length /finz.dist.
   pose proof (prog_size P). solve_addr.
 Qed.
-
 
 Lemma filter_dom_is_dom (m: gmap Addr Word) (d: gset Addr):
   d ⊆ dom (gset Addr) m →
@@ -41,7 +68,6 @@ Proof.
     eapply elem_of_gmap_dom in Hd as [? ?]. eexists. split; eauto. }
   { destruct H as [? [? ?] ]; auto. }
 Qed.
-
 
 Program Definition all_cores :=
   finz.seq
@@ -59,8 +85,11 @@ Definition core_zero := (finz.FinZ 0
                            all_cores_obligation_1
                            all_cores_obligation_2).
 
-Definition is_initial_memory (mem_frags : list prog) (m: gmap Addr Word) :=
-  let region_list := map (fun f => prog_region f) mem_frags in
+Definition is_initial_memory
+  (mem_frags : list prog) (adv_frags : list adv_prog) (m: gmap Addr Word) :=
+  let prog_list := map (fun f => prog_region f) mem_frags in
+  let adv_list := map (fun f => adv_region f) adv_frags in
+  let region_list := prog_list ∪ adv_list in
   ⋃ region_list ⊆ m /\ disjoint_list_map region_list.
 
 Definition is_initial_registers
@@ -71,9 +100,14 @@ Definition is_initial_registers
                      ∃ (w:Word), reg !! (i, r) = Some w ∧ is_cap w = false).
 
 Definition is_initial_registers_with_adv
-  (P A : prog)
-  (r_adv : RegName)
-  (reg: gmap (CoreN * RegName) Word) (i:CoreN) :=
+  (P A : prog) (r_adv : RegName) (reg: gmap (CoreN * RegName) Word) (i:CoreN) :=
   is_initial_registers P reg i
   /\ reg !! (i, r_adv) = Some (WCap RWX (prog_start A) (prog_end A) (prog_start A)) (* adversary *)
   /\ PC ≠ r_adv.
+
+Definition is_initial_registers_adv
+  (P : adv_prog) (reg: gmap (CoreN * RegName) Word) (i:CoreN) :=
+  reg !! (i, PC) = Some (WCap RWX (adv_start P) (adv_end P) (adv_start P))  (* PC *)
+  ∧ dom (gset (CoreN*RegName)) reg ⊆ (set_map (fun r => (i,r)) all_registers_s)
+  /\ (∀ (r: RegName), (i, r) ∉ ({[ (i, PC) ]} : gset (CoreN * RegName)) →
+                     ∃ (w:Word), reg !! (i, r) = Some w ∧ is_cap w = false).
